{
 "cells": [
  {
   "cell_type": "markdown",
   "metadata": {},
   "source": [
    "# MATH50003 Numerical Analysis (2022–23)\n",
    "# Problem Sheet 9\n",
    "\n",
    "\n",
    "\n",
    "This problem sheet explores Fourier interpolation, orthogonal polynomial properties and classical orthogonal polynomials.\n",
    "\n",
    "\n",
    "----\n",
    "\n",
    "**Problem 1** For the general (non-Taylor) case and $n = 2m+1$, prove that the approximate Fourier series\n",
    "$$\n",
    "f_{-m:m}(θ) := ∑_{k=-m}^m f̂_k^n {\\rm e}^{{\\rm i} k θ}\n",
    "$$\n",
    "interpolates $f$ at $θ_j = 2 π j/n$:\n",
    "$$\n",
    "f_{-m:m}(θ_j) = f(θ_j).\n",
    "$$\n",
    "Hint: show that $f_{-m:m}(θ_j) = f_n(θ_j)$, where $f_n(θ)$ is the approximate Fourier–Taylor series.\n",
    "\n",
    "**SOLUTION**\n",
    "\n",
    "We have\n",
    "$$\n",
    "{\\rm e}^{{\\rm i} k θ_j} = {\\rm e}^{2π {\\rm i} j k θ/n} = {\\rm e}^{2π {\\rm i} j (k+n) θ/n} = {\\rm e}^{{\\rm i} (k+n) θ_j}\n",
    "$$\n",
    "Combined with $f̂_k^n = f̂_{k+n}^n$ we have\n",
    "$$\n",
    "∑_{k=-m}^{-1} f̂_k^n {\\rm e}^{{\\rm i} k θ_j} = ∑_{k=-m}^{-1} f̂_{k+n}^n {\\rm e}^{{\\rm i} (k+n) θ_j} = \n",
    "∑_{k=n-m}^{n-1} f̂_k^n {\\rm e}^{{\\rm i} k θ_j} = ∑_{k=m+1}^{n-1} f̂_k^n {\\rm e}^{{\\rm i} k θ_j}.\n",
    "$$\n",
    "Thus\n",
    "$$\n",
    "f_{-m:m}(θ_j) = ∑_{k=0}^{n-1} f̂_k^n {\\rm e}^{{\\rm i} k θ_j} = f_n(θ_j) = f(θ_j).\n",
    "$$\n",
    "\n",
    "\n",
    "**END**\n",
    "\n",
    "-----\n",
    "\n",
    "\n",
    "\n",
    "**Problem 2** Construct  $π_0(x),π_1(x),π_2(x),π_3(x)$, monic OPs\n",
    "for the weights $\\sqrt{1-x^2}$ and $1-x$ on $[-1,1]$.\n",
    "Hint: for the first weight, first compute $\\int_{-1}^1 x^k \\sqrt{1-x^2} {\\rm d} x$ for $0 ≤ k ≤ 2$\n",
    "using a change-of-variables.\n",
    "\n",
    "**SOLUTION**\n",
    "\n",
    "Following the hint, we first calculate $\\int_{-1}^1 x^k\\sqrt{1-x^2}{\\rm d}x$. By symmetry, it's zero when $k$ is odd and double the integral on $[0,1]$ when $k$ is even. \n",
    "\n",
    "$$\n",
    "\\underbrace{\\int_0^1 x^k\\sqrt{1-x^2}{\\rm d}x}_{I_k} = _{x=\\sin t}\\underbrace{\\int_0^{π/2}\\sin^k(t)\\cos^2(t){\\rm d}t}_{I_k}=\\underbrace{\\int_0^{π/2}\\sin^k t{\\rm d}t}_{J_k}-\\underbrace{\\int_0^{π/2}\\sin^{k+2}t{\\rm d}t}_{J_{k+2}}.\n",
    "$$\n",
    "\n",
    "Meanwhile, \n",
    "$$J_k=-\\int_0^{π/2}\\sin^{k-1}t{\\rm d}(\\cos t)=_{\\text{integral by part}}(k-1)I_{k-2}.$$\n",
    "\n",
    "Putting the above 2 equations together, we have $I_k=(k-1)I_{k-2}-(k+1)I_k$, so $I_k=\\frac{k-1}{k+2}I_{k-2}$. Since $I_0=π/4$, we have $I_k=\\frac{(k-1)!!}{(k+2)!!}\\frac{π}{2}$ for positive even $k$. (Note that the denominator multiplies to 4, not to 2.) Keep in mind that the integral we want is double this value when $k$ is even.\n",
    "\n",
    "【Remark】Check the [beta function](https://en.wikipedia.org/wiki/Beta_function).\n",
    "\n",
    "Let $p_0(x)=1$, then $\\|p_0\\|^2=2I_0=π/2$. We know from the 3-term recurrence that\n",
    "$$xp_0(x)=a_0p_0(x)+p_1(x)$$\n",
    "where\n",
    "$$\n",
    "a_0=\\frac{⟨ p_0,xp_0⟩}{\\|p_0\\|^2}=0.$$\n",
    "Thus $p_1(x)=x$ and $\\|p_1\\|^2=2I_2=π/8$.\n",
    "From\n",
    "$$xp_1(x)=c_0p_0(x)+a_1p_1(x)+p_2(x)$$\n",
    "we have\n",
    "$$c_0=\\frac{⟨ p_0,xp_1⟩}{\\|p_0\\|^2}=2I_2/2I_0=1/4$$\n",
    "$$a_1=\\frac{⟨ p_1,xp_1⟩}{\\|p_1\\|^2}=0$$\n",
    "$$p_2(x)=xp_1(x)-c_0-a_1p_1(x)=x^2-1/4$$\n",
    "$$\\|p_2\\|^2=2I_4-I_2+1/8I_0=π/32$$\n",
    "Finally, from\n",
    "$$xp_2(x)=c_1p_1(x)+a_2p_2(x)+p_3(x)$$\n",
    "we have\n",
    "$$c_1=\\frac{⟨ p_1,xp_2⟩}{\\|p_1\\|^2}=(2I_4-1/2I_2)/(π/8)=1/4$$\n",
    "$$a_2=\\frac{⟨ p_2,xp_2⟩}{\\|p_2\\|^2}=0$$\n",
    "$$p_3(x)=xp_2(x)-c_1p_1(x)-a_2p_2(x)=x^3-1/2x$$\n",
    "\n",
    "**END**\n",
    "\n",
    "\n",
    "-------\n",
    "\n",
    "\n",
    "**Problem 3.1** Prove Theorem III.3.1: a precisely degree $n$ polynomial\n",
    "$$\n",
    "p(x) = k_n x^n + O(x^{n-1})\n",
    "$$\n",
    "satisfies\n",
    "$$\n",
    "⟨p,f_m⟩ = 0\n",
    "$$\n",
    "for all  polynomials $f_m$ of degree $m < n$ of degree less than $n$ if and only if $p(x) = c π_n$ for some constant\n",
    "$c$, where $π_n$ are monic orthogonal polynomials.\n",
    "\n",
    "\n",
    "**SOLUTION**\n",
    "As $\\{π_0,…,π_n\\}$ are a basis of all polynomials of degree $n$,\n",
    "we can write\n",
    "$$\n",
    "r(x) = ∑_{k=0}^m a_k π_k(x)\n",
    "$$\n",
    "Thus if $p(x) = c π_n(x)$, by linearity of inner products we have\n",
    "$$\n",
    "⟨p,r⟩ = ⟨cπ_n,∑_{k=0}^m a_k π_k⟩ = ∑_{k=0}^m ca_k ⟨π_n, π_k⟩ = 0.\n",
    "$$\n",
    "\n",
    "Now suppose\n",
    "$$\n",
    "p(x) = c x^n + O(x^{n-1})\n",
    "$$\n",
    "and consider $p(x) - c π_n(x)$ which is of degree $n-1$. It satisfies\n",
    "for $k ≤ n-1$\n",
    "$$\n",
    "⟨π_k, p - c π_n⟩ = ⟨π_k, p⟩ - c ⟨π_k, π_n⟩ = 0.\n",
    "$$\n",
    "Thus $p - c π_n$ is zero, i.e., $p(x) = c π_n(x)$.\n",
    "\n",
    "**END**\n",
    "\n",
    "\n",
    "**Problem 3.2 (3-term recurrence, 1st form)**\n",
    "Show that if $\\{p_n\\}$ are OPs then there exist real constants $A_n ≠ 0$, $B_n$, and $C_n$\n",
    "such that\n",
    "$$\n",
    "\\begin{align*}\n",
    "p_1(x) &= (A_0 x + B_0) p_0(x) \\\\\n",
    "p_{n+1}(x) &= (A_n x + B_n) p_n(x) - C_n p_{n-1}(x)\n",
    "\\end{align*}\n",
    "$$\n",
    "Write this as a lower triangular linear system, given $p_0(x) = \\mu \\in \\mathbb{R}$:\n",
    "$$\n",
    "L_x \\begin{bmatrix} p_0(x) \\\\ \\vdots \\\\ p_{n+1}(x) \\end{bmatrix} = \\begin{bmatrix} \\mu \\\\ 0 \\\\ \\vdots \\\\ 0 \\end{bmatrix}\n",
    "$$\n",
    "What are the bandwidths of $L_x$?\n",
    "\n",
    "**SOLUTION**\n",
    "\n",
    "The 2nd form of 3-term recurrence is\n",
    "$$xp_0(x)=a_0p_0(x)+b_0p_1(x)$$\n",
    "and\n",
    "$$xp_n(x)=c_{n-1}p_{n-1}(x)+a_np_n(x)+b_np_{n+1}(x)$$\n",
    "which is equivalent to\n",
    "$$p_1(x)=\\left(\\frac{1}{b_0}x-\\frac{a_0}{b_0}\\right)p_0(x),$$\n",
    "$$p_{n+1}(x)=\\left(\\frac{1}{b_n}x-\\frac{a_n}{b_n}\\right)p_n(x)-\\frac{c_{n-1}}{b_n}p_{n-1}(x).$$\n",
    "So we have $A_n=1/b_n$, $B_n=-\\frac{a_n}{b_n}$ and $C_n=\\frac{c_{n-1}}{b_n}$.\n",
    "\n",
    "Writing down the recurrence for every $n$, we have a lower tridiagonal linear system\n",
    "$$\n",
    "\\underbrace{\\begin{bmatrix}\n",
    "1 &&&&\\\\\n",
    "-A_0x-B_0 & 1 &&&\\\\\n",
    "C_1 & -A_1x-B_1 & 1 &&\\\\\n",
    "& \\ddots &\\ddots&\\ddots&\\\\\n",
    "&&C_{n}&-A_nx-B_n&1\n",
    "\\end{bmatrix}}_{L_x}\n",
    "\\underbrace{\\begin{bmatrix} p_0(x) \\\\ \\vdots \\\\ p_{n+1}(x) \\end{bmatrix}}_{\\mathbf{P}(x)} = \\underbrace{\\begin{bmatrix} μ \\\\ 0 \\\\ \\vdots \\\\ 0 \\end{bmatrix}}_{\\mu\\mathbf{e}_1}\n",
    "$$\n",
    "\n",
    "The bandwidths are $(ℓ,u) = (2,0)$ (lower tridiagonal).\n",
    "\n",
    "**END**\n",
    "\n",
    "**Problem 3.3** If $w(-x) = w(x)$ for a weight supported on $[-b,b]$ show that $a_n = 0$.\n",
    "Hint: first show that the (monic) polynomials $p_{2n}(x)$ are even and $p_{2n+1}(x)$ are odd.\n",
    "\n",
    "**SOLUTION**\n",
    "\n",
    "An integral is zero if its integrand is odd. \n",
    "Moreover an even function times an odd function is odd and\n",
    "an odd function times an odd fuction is even.\n",
    "Note that $p_0(x)$ and $w(x)$ are even and $x$ is odd. \n",
    "\n",
    "We see that $a_0$ is zero:\n",
    "$$\n",
    "⟨p_0,x p_0(x)⟩ = \\int_{-b}^b x w(x) {\\rm d} x = 0\n",
    "$$\n",
    "since $xw(x)$ is odd,\n",
    "which shows that\n",
    "$$\n",
    "p_1(x) = xp_0(x)\n",
    "$$\n",
    "is odd. We now proceed by induction. Assume that $p_{2n}$ is even and $p_{2n-1}$ is odd.\n",
    "We have:\n",
    "$$\n",
    "⟨p_{2n},x p_{2n}(x)⟩ = \\int_{-b}^b x w(x) p_{2n}(x)^2 {\\rm d} x = 0\n",
    "$$\n",
    "since $x w(x) p_{2n}(x)^2$ is odd, therefore $a_{2n} = 0$.\n",
    "Thus from\n",
    "$$\n",
    "p_{2n+1}(x) = (x p_{2n}(x)- c_{2n-1} p_{2n-1}(x)) / b_{2n} \n",
    "$$\n",
    "we see that $p_{2n+1}$ is odd. Then\n",
    "$$\n",
    "⟨p_{2n+1},x p_{2n+1}(x)⟩ = \\int_{-b}^b x w(x) p_{2n+1}(x)^2 {\\rm d} x = 0\n",
    "$$\n",
    "since $x w(x) p_{2n+1}(x)^2$ is odd, therefore $a_{2n+1} = 0$.\n",
    "and hence\n",
    "$$\n",
    "p_{2n+2}(x) = (x p_{2n+1}(x)- c_{2n} p_{2n}(x)) / b_{2n+1} \n",
    "$$\n",
    "is even.\n",
    "\n",
    "\n",
    "\n",
    "**END**\n",
    "\n",
    "----\n",
    "\n",
    "**Problem 4.1** Recall  the Chebyshev polynomials $T_0(x) = 1$, $T_n(x)  = 2^{n-1} x^n + O(x^{n-1})$ which are orthogonal with\n",
    "respect to $1/\\sqrt{1-x^2}$ and $U_n(x) = 2^n x^n +O(x^{n-1})$ which are orthogonal with respect to $\\sqrt{1-x^2}$, both on $[-1,1]$. \n",
    "Use the fact that orthogonal polynomials are uniquely determined by their leading order coefficient and orthogonality to lower \n",
    "dimensional polynomials to show that:\n",
    "$$\n",
    "T_n'(x) = n U_{n-1}(x).\n",
    "$$\n",
    "Hint: use integration-by-parts.\n",
    "\n",
    "\n",
    "**SOLUTION**\n",
    "\n",
    "We need to verify that $T_n'(x)$\n",
    "1. graded polynomials\n",
    "2. orthogonal w.r.t. $\\sqrt{1-x^2}$ on $[-1,1]$, and\n",
    "3. have the leading coefficient $n 2^n$.\n",
    "(1) and (3) are clear:\n",
    "$$\n",
    "T_n'(x) = n 2^{n-1} x^{n-1} + O(x^{n-2}).\n",
    "$$\n",
    "(2) For $f_m$ degree $m < n-1$ we have\n",
    "$$\n",
    "∫_{-1}^1 T_n'(x) f_m(x) \\sqrt{1-x^2} {\\rm d}x = \n",
    "-∫_{-1}^1 T_n(x) \\underbrace{(f_m'(x)(1-x^2) -x f_m)}_{\\hbox{degree $m+1 < n$}}  (1-x^2)^{-1/2} {\\rm d}x = 0.\n",
    "$$\n",
    "\n",
    "\n",
    "\n",
    "**END**\n",
    "\n",
    "**Problem 4.2** Prove that\n",
    "$$\n",
    "U_n(\\cos θ) = {\\sin(n+1) θ \\over \\sin θ}.\n",
    "$$\n",
    "\n",
    "\n",
    "**SOLUTION**\n",
    "\n",
    "We need to verify\n",
    "$$\n",
    "p_n(x) := {\\sin(n+1) θ \\over \\sin θ}\n",
    "$$\n",
    "are\n",
    "1. graded polynomials\n",
    "2. orthogonal w.r.t. $\\sqrt{1-x^2}$ on $[-1,1]$, and\n",
    "3. have the leading coefficient $2^n$.\n",
    "Then uniqueness will guarantee that $p_n(x) = U_n(x)$.\n",
    "\n",
    "(2) follows under a change of variables\n",
    "$$\n",
    "\\begin{align*}\n",
    "\\int_{-1}^1 p_n(x)p_m(x)\\sqrt{1-x^2}{\\rm d}x &= \\int_0^{π}p_n(\\cos θ)p_m(\\cos θ)\\sin^2 θ{\\rm d} θ \\\\\n",
    "&= \\int_0^{π}\\sin(n+1) θ\\sin(m+1) θ{\\rm d} θ=\\frac{π}{2}δ_{mn}\n",
    "\\end{align*}\n",
    "$$\n",
    "where the last step can be shown by substituting $\\sin kθ = (\\exp(ikθ)-\\exp(-ikθ)/(2i)$.\n",
    "\n",
    "To see that they are graded, first note that\n",
    "$$\n",
    "p_0(x) = {\\sin θ /\\sin θ} = 1, p_1(x) =  {\\sin 2 θ \\over \\sin θ} = {2 \\sin θ \\cos θ \\over \\sin θ} = 2x.\n",
    "$$\n",
    "Now for $n = 1,2,…$  use the fact that\n",
    "$$\n",
    "xp_n(x)=\\frac{\\cos θ\\sin(n+1) θ}{\\sin θ}=\\frac{\\sin (n+2) θ+\\sin n θ}{2\\sin θ}\n",
    "$$\n",
    "In other words $2xp_n(x)=p_{n+1}(x)+p_{n-1}(x)$, i.e. $p_{n+1}(x) = 2x p_n(x) + p_{n-1}(x).\n",
    "By induction it follows that\n",
    "$$\n",
    "p_n(x) = 2^n x^n + O(x^{n-1})\n",
    "$$\n",
    "which also proves (3).\n",
    "\n",
    "\n",
    "**END**\n",
    "\n",
    "**Problem 4.3** Show that\n",
    "$$\n",
    "\\begin{align*}\n",
    "x U_0(x) &= U_1(x)/2 \\\\\n",
    "x U_n(x) &= {U_{n-1}(x) \\over 2} + {U_{n+1}(x) \\over 2}.\n",
    "\\end{align*}\n",
    "$$\n",
    "\n",
    "**SOLUTION**\n",
    "\n",
    "The first result is trivial. For the other parts, from the solution to 4.2 we know $2xU_n(x)=U_{n+1}(x)+U_{n-1}(x)$\n",
    "and this result is a reordering.\n",
    "\n",
    "**END**\n",
    "\n",
    "\n",
    "\n",
    "-----\n",
    "\n",
    "**Problem 5.1** Consider Hermite polynomials orthogonal with respect to the weight $\\exp(-x^2)$ on $ℝ$\n",
    "with the normalisation\n",
    "$$\n",
    "H_n(x) = 2^n x^n + O(x^{n-1}).\n",
    "$$\n",
    "Prove the Rodrigues formula\n",
    "$$\n",
    "H_n(x) = (-1)^n \\exp(x^2) {{\\rm d}^n \\over {\\rm d}x^n} \\exp(-x^2).\n",
    "$$\n",
    "Hint: use integration-by-parts.\n",
    "\n",
    "**SOLUTION**\n",
    "Define\n",
    "$$\n",
    "p_n(x) := (-1)^n \\exp(x^2) {{\\rm d}^n \\over {\\rm d}x^n} \\exp(-x^2)\n",
    "$$\n",
    "\n",
    "We need to verify that $p_n$\n",
    "1. are graded polynomials\n",
    "2. are orthogonal to all lower degree polynomials on $\\mathbb{R}$, and\n",
    "3. have the right leading coefficient $2^n$.\n",
    "\n",
    "Comparing the Rodrigues formula for $n$ and $n-1$, we find that \n",
    "$$\n",
    "(-1)^n\\exp(-x^2)p_n(x)={{\\rm d} \\over {\\rm d}x}\\left((-1)^{n-1}\\exp(-x^2)p_{n-1}(x)\\right)\n",
    "$$\n",
    "which reduces to\n",
    "$$p_n(x)=2xp_{n-1}(x)-p_{n-1}'(x).$$\n",
    "\n",
    "(1) and (3) then follows from induction since $p_0(x)=1$.\n",
    "\n",
    "(2) follows by integration by parts. If $r_m$ is any degree $m<n$ polynomial we have:\n",
    "$$\n",
    "\\begin{align*}\n",
    "\\int_{-∞}^∞ p_n(x)r_m(x)\\exp(-x^2){\\rm d}x&=\\int_{-∞}^∞{{\\rm d}^n \\over {\\rm d}x^n} \\exp(-x^2)r(x){\\rm d}x = -\\int_{-∞}^∞{{\\rm d}^{n-1} \\over {\\rm d}x^{n-1}} \\exp(-x^2)r'(x){\\rm d}x\\\\\n",
    "&=⋯\\text{integration by parts $n$ times}…=(-1)^n\\int_{-∞}^∞ \\exp(-x^2)r_m^{(n)}(x)=0\n",
    "\\end{align*}\n",
    "$$\n",
    "Thus $p_n(x) = H_n(x)$ by uniqueness.\n",
    "\n",
    "**END**\n",
    "\n",
    "**Problem 5.2⋆** What are $k_n^{(1)}$ and $k_n^{(2)}$ such that\n",
    "$$\n",
    "H_n(x) = 2^n x^n + k_n^{(1)} x^{n-1} + k_n^{(2)} x^{n-2} + O(x^{n-3})\n",
    "$$\n",
    "\n",
    "**SOLUTION**\n",
    "\n",
    "From Problem 3.1,\n",
    "$$H_n(x)=2xH_{n-1}(x)-H_{n-1}'(x).$$\n",
    "Thus we have\n",
    "$$k_n^{(1)}=2k_{n-1}^{(1)}$$\n",
    "$$k_n^{(2)}=2k_{n-1}^{(2)}-(n-1)2^{n-1}$$\n",
    "\n",
    "Since $k_0^{(1)}=0$, we have $k_n^{(1)}=0$. For the second recurrence, divide both sides by $2^n$:\n",
    "$$2^{-n}k_n^{(2)}=2^{-(n-1)}k_{n-1}^{(2)}-\\frac{n-1}{2}$$\n",
    "Since $k_0^{(2)}=0$, we have $2^{-n}k_n^{(2)}=-\\frac{1+⋯+(n-1)}{2}=-\\frac{n(n-1)}{4}$, so $k_n^{(2)}=-n(n-1)2^{n-2}$.\n",
    "\n",
    "**END**\n",
    "\n",
    "**Problem 5.3⋆** Deduce the 3-term recurrence relationship for $H_n(x)$.\n",
    "\n",
    "**SOLUTION**\n",
    "\n",
    "Our goal is to find $a_n$, $b_n$ and $c_n$ such that\n",
    "$$xH_n(x)=c_{n-1}H_{n-1}(x)+a_nH_n(x)+b_nH_{n+1}(x).$$\n",
    "Compare the 3 leading coefficients on both sides and use the results from Problem 3.1 and Problem 3.2:\n",
    "$$\n",
    "2^n=0+0+b_n2^{n+1}\n",
    "$$\n",
    "$$\n",
    "0=0+a_n2^n+0\n",
    "$$\n",
    "$$\n",
    "n(n-1)2^{n-2}=c_{n-1}2^{n-1}+0+b_n(n+1)n2^{n-1}\n",
    "$$\n",
    "Thus we have $b_n=1/2$, $a_n=0$ and $c_{n-1}=n$.\n",
    "\n",
    "**END**\n",
    "\n",
    "**Problem 5.4** Prove that $H_n'(x) = 2n H_{n-1}(x)$. Hint: show orthogonality of $H_n'$ to all lower degree polynomials,\n",
    "and that the normalisation constants match.\n",
    "\n",
    "**SOLUTION**\n",
    "\n",
    "We have for $f_m$ degree $m < n-1$, using integration by parts\n",
    "$$\n",
    "⟨H_n', f_m⟩ = ∫_{-∞}^∞ H_n'(x) f_m(x) {\\rm e}^{-x^2} {\\rm d} x =  ∫_{-∞}^∞ H_n(x) \\undebrace{(f_m'(x) -2x f_m)}_{degree $m+1 < n$}  {\\rm e}^{-x^2} {\\rm d} x = 0.\n",
    "$$\n",
    "Further,\n",
    "$$\n",
    "H_n'(x) = n 2^n x^{n-1} + O(x^{n-1}) = 2n (2^{n-1} x^{n-1} + O(x^{n-1}))\n",
    "$$\n",
    "hence the normalisation constants match.\n",
    "\n",
    "**END**"
   ]
  }
 ],
 "metadata": {
  "kernelspec": {
   "display_name": "Julia 1.9.0",
   "language": "julia",
   "name": "julia-1.9"
  },
  "language_info": {
   "file_extension": ".jl",
   "mimetype": "application/julia",
   "name": "julia",
   "version": "1.9.0"
  }
 },
 "nbformat": 4,
 "nbformat_minor": 2
}
